move stuff into scratch subdir

csrc/bar.c
@@ -1,5 +1,10 @@
 #include "foo.h"
 
+int x = 4;
+
 int bar(struct blah *q) {
-    return q->z;
+    if (q->z == 3) {
+    	*(int *)(q + q->w) = q->w;
+    }
+    return q->z + x;
 }
