csrc/external.h
@@ -1,0 +1,18 @@
+#ifndef EXTERNAL_H
+#define EXTERNAL_H
+
+#include <stdlib.h>
+
+struct my_lock;
+
+struct my_lock *my_lock_create(void);
+void my_lock_acquire(struct my_lock *lk);
+void my_lock_release(struct my_lock *lk);
+void my_lock_destroy(struct my_lock *lk);
+
+void *my_malloc(size_t s);
+void my_free(void *p);
+
+void my_fork(void(*foo)());
+
+#endif /* EXTERNAL_H */
